@@ -14,6 +14,7 @@ Set Default Proof Using "Type*".
 
 
 Lemma eval_SI_eval {efl : EEnvFlags} {wfl : WcbvFlags} Σ Γ e v n :
+  ~~ has_cstr_params ->
   cstr_as_blocks ->
   with_constructor_as_block ->
   ~~ with_guarded_fix ->
@@ -24,7 +25,7 @@ Lemma eval_SI_eval {efl : EEnvFlags} {wfl : WcbvFlags} Σ Γ e v n :
   eval Σ Γ e v n ->
   EWcbvEval.eval Σ (substlg (map term_of_val Γ) 0 e) (term_of_val v).
 Proof.
-  intros hCstrBlcs hCstrBlcs' h_unguarded h_app wf_Σ wf_env wf_e heval.
+  intros hCstrParams hCstrBlcs hCstrBlcs' h_unguarded h_app wf_Σ wf_env wf_e heval.
   induction heval; simple; try now econstructor.
   - econstructor.
     + now apply IHheval1; simple.
@@ -76,6 +77,7 @@ Proof.
     + apply IHheval; now simple.
     + now simple.
     + now simple.
+    + now rewrite e2; simple.
     + apply value_final, value_term_of_val; try easy.
       apply eval_SI_wellformed_val in heval; simple; try easy.
       now eapply heval, nth_error_In. 
@@ -152,127 +154,129 @@ Proof.
     + now apply IHheval2; simple.
   - unfold cunfold_cofix in heq1.
     destruct (nth_error mfix idx) eqn:heq; last easy; simple.
+    injection heq1 as ?; subst.
+    apply eval_SI_wellformed_val in heval1 as hwf; simple; last easy.
+      unfold wf_fix, test_def in hwf; simple.
+      repeat split; simple; try easy.
+    assert (forallb (wellformed_val Σ) (cofix_env mfix env ++ env)).
+    { rewrite cofix_env_map; simple.
+      intros x [(? & ? & ?%in_rev%in_seq)%in_map_iff| hIn]%in_app_iff; subst; simple; last easy.
+      simple; unfold wf_fix, test_def; simple.
+      repeat split; try easy.
+      now apply Nat.ltb_lt. }
+    assert (wellformed Σ (#|mfix| + #|env|) (mkApps (dbody d) (map term_of_val args))).
+    { rewrite wellformed_mkApps; simple; split; last first.
+      { now intros; apply wellformed_val_wellformed. }
+      now apply nth_error_In in heq. }
     eapply EWcbvEval.eval_cofix_case.
     + apply IHheval1; now simple.
     + unfold EGlobalEnv.cunfold_cofix; simple.
       reflexivity.
-    + apply eval_SI_wellformed_val in heval1 as hwf; simple; last easy.
-      unfold wf_fix, test_def in hwf; simple.
-      unshelve epose proof IHheval2 _ _; simple; try easy.
-      { repeat split; simple; try easy.
-        rewrite wellformed_mkApps; simple; split; last first.
-        { now intros; apply wellformed_val_wellformed. }
-        apply wellformed_substl; simple.
-        - rewrite cofix_env_map map_map_compose.
-          intros x [(? & ? & hIn%in_rev%in_seq)%in_map_iff| (? & ? & hIn)%in_map_iff]%in_app_iff; subst;
-            apply wellformed_val_wellformed; try easy.
-          simple; unfold wf_fix, test_def; simple; repeat split; try easy.
-          now apply Nat.ltb_lt.
-        - injection heq1 as ?; subst.
-          apply nth_error_In in heq.
-          now eapply wellformed_up. }
+    + unshelve epose proof IHheval2 _ _; simple; try easy.
+      eapply EWcbvEval.eval_iota_block; simple; try easy.
+      { lazymatch goal with
+        | h: EWcbvEval.eval _ ?e1 (tConstruct _ _ _)
+          |- EWcbvEval.eval _ ?e2 (tConstruct _ _ _) =>
+            assert (e1 = e2) as <-; last easy
+        end.
+        simple. f_equal; last first.
+        - rewrite map_map_compose.
+          apply All_map_eq. simple.
+          intros arg hIn.
+          assert (closed (term_of_val arg)) as h_closed.
+          { now eapply wellformed_closed, wellformed_val_wellformed.  }
+          now eapply substlg_closed.
+        - rewrite cofix_subst_map cofix_env_map. simple.
+          rewrite -substlg_app; simple.
+          { intros ? ?%in_rev%in_seq.
+            simple. intros ? ?.
+            unfold test_def.
+            apply closed_substlg; simple; last now eapply wellformed_closed.
+            intros ? (? & ? & ?)%in_map_iff ?; subst.
+            now eapply wellformed_closed, wellformed_val_wellformed. }
+          { intros. now eapply wellformed_closed, wellformed_val_wellformed. }
+          f_equal. rewrite map_map_compose.
+          apply map_ext.
+          intros; simple.
+          reflexivity. }
+      { now simple. }
+      { now simple. }
+      unshelve epose proof IHheval3 _ _; simple; try easy.
+      { intros ? [?%in_rev | ?]%in_app_iff; last easy.
+        now apply eval_SI_wellformed_val in heval2; simple. }
+      { rewrite heq5. now apply nth_error_In in heq3. }
       lazymatch goal with
       | h: EWcbvEval.eval _ ?e1 (term_of_val _)
-        |- EWcbvEval.eval _ ?e2 _ =>
+        |- EWcbvEval.eval _ ?e2 (term_of_val _) =>
           assert (e1 = e2) as <-; last easy
       end.
-      do 2 f_equal; last first.
-      { rewrite map_map_compose.
-        apply All_map_eq. simple.
-        intros arg hIn.
-        assert (closed (term_of_val arg)) as h_closed.
-        { now eapply wellformed_closed, wellformed_val_wellformed.  }
-        now eapply substlg_closed. }
-      injection heq1 as ?; subst.
-      rewrite cofix_subst_map cofix_env_map. simple.
-      assert (#|mfix| = #|map (tCoFix (map (map_def (substlg (map term_of_val env) #|mfix|)) mfix)) (List.rev (seq 0 #|mfix|))| + 0) as h by now simple.
-      rewrite {4}h.
-      rewrite substlg_app; simple.
-      { intros ? ?%in_rev%in_seq.
-        simple. intros ? ?.
-        unfold test_def.
-        apply closed_substlg; simple; last now eapply wellformed_closed.
-        intros ? (? & ? & ?)%in_map_iff ?; subst.
+      unfold iota_red; simple.
+      rewrite -substlg_app.
+      { apply eval_SI_wellformed_val in heval2; simple; try easy.
+        intros x hIn%in_rev. now eapply wellformed_closed, wellformed_val_wellformed. }
+      { simple. intros ? ?.
         now eapply wellformed_closed, wellformed_val_wellformed. }
-      { intros. now eapply wellformed_closed, wellformed_val_wellformed. }
-      erewrite substlg_closed; last reflexivity; last first.
-      { apply closed_substlg; simple; last first.
-        { eapply wellformed_closed. now apply nth_error_In in heq. }
-        intros x [(? & ? & (? & ? & hIn%in_rev%in_seq)%in_map_iff)%in_map_iff | (? & ? & hIn)%in_map_iff]%in_app_iff k;
-          subst; eapply wellformed_closed, wellformed_val_wellformed; try easy.
-        simple; unfold wf_fix; simple; repeat split; try easy.
-        now apply Nat.ltb_lt. } 
-      do 2 f_equal.
-      rewrite map_map_compose.
-      apply map_ext.
-      intros; simple.
-      reflexivity.
-
+      do 2 f_equal; now simple.
   - unfold cunfold_cofix in heq1.
     destruct (nth_error mfix idx) eqn:heq; last easy; simple.
+    injection heq1 as ?; subst.
+    apply eval_SI_wellformed_val in heval1 as hwf; simple; last easy.
+      unfold wf_fix, test_def in hwf; simple.
+      repeat split; simple; try easy.
+    assert (forallb (wellformed_val Σ) (cofix_env mfix env ++ env)).
+    { rewrite cofix_env_map; simple.
+      intros x [(? & ? & ?%in_rev%in_seq)%in_map_iff| hIn]%in_app_iff; subst; simple; last easy.
+      simple; unfold wf_fix, test_def; simple.
+      repeat split; try easy.
+      now apply Nat.ltb_lt. }
+    assert (wellformed Σ (#|mfix| + #|env|) (mkApps (dbody d) (map term_of_val args))).
+    { rewrite wellformed_mkApps; simple; split; last first.
+      { now intros; apply wellformed_val_wellformed. }
+      now apply nth_error_In in heq. }
     eapply EWcbvEval.eval_cofix_proj.
     + apply IHheval1; now simple.
     + unfold EGlobalEnv.cunfold_cofix; simple.
       reflexivity.
-    + apply eval_SI_wellformed_val in heval1 as hwf; simple; last easy.
-      unfold wf_fix, test_def in hwf; simple.
-      unshelve epose proof IHheval2 _ _; simple; try easy.
-      { repeat split; simple; try easy.
-        rewrite wellformed_mkApps; simple; split; last first.
-        { now intros; apply wellformed_val_wellformed. }
-        apply wellformed_substl; simple.
-        - rewrite cofix_env_map map_map_compose.
-          intros x [(? & ? & hIn%in_rev%in_seq)%in_map_iff| (? & ? & hIn)%in_map_iff]%in_app_iff; subst;
-            apply wellformed_val_wellformed; try easy.
-          simple; unfold wf_fix, test_def; simple; repeat split; try easy.
-          now apply Nat.ltb_lt.
-        - injection heq1 as ?; subst.
-          apply nth_error_In in heq.
-          now eapply wellformed_up. }
-      lazymatch goal with
-      | h: EWcbvEval.eval _ ?e1 (term_of_val _)
-        |- EWcbvEval.eval _ ?e2 _ =>
-          assert (e1 = e2) as <-; last easy
-      end.
-      do 2 f_equal; last first.
-      { rewrite map_map_compose.
-        apply All_map_eq. simple.
-        intros arg hIn.
-        assert (closed (term_of_val arg)) as h_closed.
-        { now eapply wellformed_closed, wellformed_val_wellformed.  }
-        now eapply substlg_closed. }
-      injection heq1 as ?; subst.
-      rewrite cofix_subst_map. simple.
-      assert (#|mfix| = #|map (tCoFix (map (map_def (substlg (map term_of_val env) #|mfix|)) mfix)) (List.rev (seq 0 #|mfix|))| + 0) as h by now simple.
-      rewrite {3}h.
-      rewrite substlg_app; simple.
-      { intros ? ?%in_rev%in_seq.
-        simple. intros ? ?.
-        unfold test_def.
-        apply closed_substlg; simple; last now eapply wellformed_closed.
-        intros ? (? & ? & ?)%in_map_iff ?; subst.
-        now eapply wellformed_closed, wellformed_val_wellformed. }
-      { intros. now eapply wellformed_closed, wellformed_val_wellformed. }
-      erewrite substlg_closed; last reflexivity; last first.
-      { apply closed_substlg; simple; last first.
-        { eapply wellformed_closed. now apply nth_error_In in heq. }
-        rewrite cofix_env_map map_map_compose.
-        intros ? [(? & ? & hIn%in_rev%in_seq)%in_map_iff | (? & ? & hIn)%in_map_iff]%in_app_iff ?; subst;
-          eapply wellformed_closed, wellformed_val_wellformed; try easy.
-        simple; unfold wf_fix; simple; repeat split; try easy.
-        now apply Nat.ltb_lt. } 
-      do 2 f_equal.
-      rewrite cofix_env_map map_map_compose.
-      apply map_ext.
-      intros; simple.
-      reflexivity.
+    + unshelve epose proof IHheval2 _ _; simple; try easy.
+      eapply EWcbvEval.eval_proj_block; simple; try easy.
+      { lazymatch goal with
+        | h: EWcbvEval.eval _ ?e1 (tConstruct _ _ _)
+          |- EWcbvEval.eval _ ?e2 (tConstruct _ _ _) =>
+            assert (e1 = e2) as <-; last easy
+        end.
+        simple. f_equal; last first.
+        - rewrite map_map_compose.
+          apply All_map_eq. simple.
+          intros arg hIn.
+          assert (closed (term_of_val arg)) as h_closed.
+          { now eapply wellformed_closed, wellformed_val_wellformed.  }
+          now eapply substlg_closed.
+        - rewrite cofix_subst_map cofix_env_map. simple.
+          rewrite -substlg_app; simple.
+          { intros ? ?%in_rev%in_seq.
+            simple. intros ? ?.
+            unfold test_def.
+            apply closed_substlg; simple; last now eapply wellformed_closed.
+            intros ? (? & ? & ?)%in_map_iff ?; subst.
+            now eapply wellformed_closed, wellformed_val_wellformed. }
+          { intros. now eapply wellformed_closed, wellformed_val_wellformed. }
+          f_equal. rewrite map_map_compose.
+          apply map_ext.
+          intros; simple.
+          reflexivity. }
+      { now simple. }
+      { rewrite heq2. now simple. }
+      apply value_final, value_term_of_val; simple.
+      apply nth_error_In in heq5.
+      now apply eval_SI_wellformed_val in heval2; simple.
   - econstructor; try easy.
     apply IHheval; try easy.
     pose proof lookup_env_wellformed wf_Σ isdecl.
     simple.
   - rewrite /lookup_constructor_pars_args e /= in wf_e.
-    econstructor; simple; try easy.
     rewrite hCstrBlcs in wf_e; simple.
+    econstructor; simple; try easy.
+    { symmetry. now apply eqb_eq. }
     clear l.
     destruct wf_e as [_ [_ wf_e]]. induction a; simple; try easy.
     destruct IHa.
